theories/modules/Sp.v
@@ -1,10 +1,29 @@
 Require Export Common FSpec Fn.
 From iris.proofmode Require Import proofmode.
 
-Global Notation specmap := (gmap (option fname) fspec_rel).
+(* Global Notation specmap := ((gmap fname fspec_rel) * bool)%type. *)
+Definition specmap `{Σ: GRA} : Type := (gmap fname fspec_rel) * bool.
 
 Variant fn_has_spec_in `{Σ : GRA} (sp : specmap) (f : string) (fsp : fspec) : Prop :=
 | fn_has_spec_in_intro fsp2
-    (SPEC: sp !! Some (fid f) = fsp_some fsp2)
+    (SPEC: sp.1 !! fid f = fsp_some fsp2)
     (WEAK : ⊢ fspec_imply fsp2 fsp).
 Hint Constructors fn_has_spec_in : core.
+
+Definition gmap_to_specmap `{Σ: GRA} (m : gmap fname fspec_rel) : specmap := (m, false).
+#[warnings="-uniform-inheritance"]
+Coercion gmap_to_specmap : gmap >-> specmap.
+
+Global Instance specmap_empty `{Σ: GRA} : Empty specmap := (∅, false).
+
+Global Instance specmap_union `{Σ: GRA} : Union specmap :=
+  λ sp sp', (sp.1 ∪ sp'.1, sp.2 || sp'.2).
+
+Global Instance specmap_subseteq `{Σ: GRA} : SubsetEq specmap :=
+  λ sp sp', sp.1 ⊆ sp'.1 ∧ (sp.2 → sp'.2).
+
+Global Instance specmap_subseteq_reflexive `{Σ: GRA} : Reflexive (specmap_subseteq).
+Proof. intros []. split; et. Qed.
+
+Global Instance specmap_subseteq_transitive `{Σ: GRA} : Transitive (specmap_subseteq).
+Proof. intros [] [] [] [] []. ss. split; et. etrans; et. Qed.
