theories/cancellation/Cancel.v
@@ -114,7 +114,7 @@ Module Cancel. Section Cancel.
     (WFS: SMod.cancellable md)
     (WF: Mod.wf (SMod.to_mod ∅ (SMod.cancel md)))
     (VALID: ✓ rs)
-    (MAIN : ∃ P Q, (fspec_flat (SMod.conc_sp_from md !! Some entry)) P Q ∧
+    (MAIN : ∃ P Q, (fspec_flat ((SMod.conc_sp_from md).1 !! entry)) P Q ∧
       (Own rs ⊢ |==> (P tt↑ tt↑ ∗ Own rt) ∗ TIDAUTH 0 ∗ YIELDAUTH 1) ∧
       ∀ varg arg, Q varg arg ⊢ ⌜varg = arg⌝)
     :
@@ -153,12 +153,9 @@ Module Cancel. Section Cancel.
     eapply gsim_tau_src; ss; [do 2 f_equal; hnorm_itr|]. ghnorm_l. rewrite bind_ret_r.
 
     destruct fspo as [fsp|]; ss.
-    { assert (Hf : SMod.sp_from md !! Some entry = Some fsp).
-      { rewrite /SMod.sp_from lookup_kmap_Some; exists entry; split; ss.
-        rewrite !lookup_omap lookup_fmap lookup_omap FIND0 //.
-      }
-      rewrite /SMod.conc_sp_from lookup_insert_ne // Hf /= in MAIN.
-      destruct MAIN as [P [Q [Hfsp [Hp Hq]]]].
+    { assert (Hf : (SMod.sp_from md).1 !! entry = Some fsp).
+      { rewrite !lookup_omap lookup_fmap lookup_omap FIND0 //. }
+      rewrite Hf /= in MAIN. destruct MAIN as [P [Q [Hfsp [Hp Hq]]]].
       eapply gsim_Take_tgt; ss; [do 2 f_equal; hnorm_itr|]. exists (FSpec_mk _ _ Hfsp).
       eapply gsim_tau_tgt; [s; do 2 f_equal; hnorm_itr|]. ss.
       eapply gsim_Take_tgt; ss; [do 2 f_equal; hnorm_itr|]. exists (tt↑).
@@ -208,7 +205,7 @@ Module Cancel. Section Cancel.
 
     Lemma cancellation md IC Pinit :
       SMod.cancellable md →
-      (∃ P Q, (fspec_flat (SMod.conc_sp_from md !! Some entry)) P Q ∧
+      (∃ P Q, (fspec_flat ((SMod.conc_sp_from md).1 !! entry)) P Q ∧
         (TID 0 ∗ YIELD 0 ∗ winv (⊤, ⊤) ∗ Pinit ⊢ |==> (P tt↑ tt↑)) ∧
         ∀ varg arg, Q varg arg ⊢ ⌜varg = arg⌝) →
       refines
