theories/simulations/msim/TacticsCommon.v
@@ -514,10 +514,10 @@ Ltac clear_st :=
 
 Ltac simpl_sp :=
   try match goal with
-  | H : ?sp1 ⊆ ?sp2 |- context [?sp2 !! ?key] =>
-    unshelve erewrite (lookup_weaken sp1 sp2 key _ _ H);
+   | H : ?sp1 ⊆ ?sp2 |- context [?sp2.1 !! ?key] =>
+    unshelve erewrite (lookup_weaken sp1.1 sp2.1 key _ _ (proj1 H));
     [|simpl_map; reflexivity|]
-  end.
+   end.
 
 (* Normalization tactics *)
 Ltac replace_l :=
